fixes to uints

ulib/FStar.UInt16.fst
@@ -2,16 +2,16 @@ module FStar.UInt16
 
 let n = 16
 
-open FStar.Int
+open FStar.UInt
 open FStar.Mul
 
 (* NOTE: anything that you fix/update here should be reflected in [FStar.UIntN.fstp], which is mostly
  * a copy-paste of this module. *)
 
-private type t' = | Mk: v:int_t n -> t'
+private type t' = | Mk: v:uint_t n -> t'
 type t = t'
 
-let v (x:t) : Tot (int_t n) = x.v
+let v (x:t) : Tot (uint_t n) = x.v
 
 val add: a:t -> b:t -> Pure t
   (requires (size (v a + v b) n))
@@ -28,7 +28,7 @@ let add_underspec a b =
 
 val add_mod: a:t -> b:t -> Pure t
   (requires True)
-  (ensures (fun c -> (v a + v b) @% pow2 n = v c))
+  (ensures (fun c -> (v a + v b) % pow2 n = v c))
 let add_mod a b =
   Mk (add_mod (v a) (v b))
 
@@ -48,7 +48,7 @@ let sub_underspec a b =
 
 val sub_mod: a:t -> b:t -> Pure t
   (requires True)
-  (ensures (fun c -> (v a - v b) @% pow2 n = v c))
+  (ensures (fun c -> (v a - v b) % pow2 n = v c))
 let sub_mod a b =
   Mk (sub_mod (v a) (v b))
 
@@ -68,7 +68,7 @@ let mul_underspec a b =
 
 val mul_mod: a:t -> b:t -> Pure t
   (requires True)
-  (ensures (fun c -> (v a * v b) @% pow2 n = v c))
+  (ensures (fun c -> (v a * v b) % pow2 n = v c))
 let mul_mod a b =
   Mk (mul_mod (v a) (v b))
 
@@ -103,20 +103,20 @@ let logor a b = Mk (logor (v a) (v b))
 val lognot: t -> Tot t
 let lognot a = Mk (lognot (v a))
 
-val int_to_t: x:(int_t n) -> Pure t
+val uint_to_t: x:(uint_t n) -> Pure t
   (requires True)
   (ensures (fun y -> v y = x))
-let int_to_t x = Mk (to_int_t n x)
+let uint_to_t x = Mk (to_uint_t n x)
 
 (* Shift operators *)
 val shift_right: a:t -> s:nat -> Pure t
   (requires True)
-  (ensures (fun c -> v c = (v a /% (pow2 s))))
+  (ensures (fun c -> v c = (v a / (pow2 s))))
 let shift_right a s = Mk (shift_right (v a) s)
 
 val shift_left: a:t -> s:nat -> Pure t
   (requires True)
-  (ensures (fun c -> v c = ((v a * pow2 s) @% pow2 n)))
+  (ensures (fun c -> v c = ((v a * pow2 s) % pow2 n)))
 let shift_left a s = Mk (shift_left (v a) s)
 
 (* Comparison operators *)
